Mica/SeparationLogic/Axioms.lean
@@ -163,17 +163,10 @@ theorem wp.letIn {b : Runtime.Binder} {bound body : Runtime.Expr} {Q : Runtime.V
   isplitl []
   · iintro %v Hv
     iapply wp.func
-    iapply (@wp.fix .none [b] body Q
-      (fun vs => ∃ v', ⌜vs = [v']⌝ ∗ wp (body.subst (Runtime.Subst.id.update' b v')) Q))
-    · iintro _IH %vs ⟨%v', %Heq, Hwp⟩
-      subst Heq
-      simp only [Runtime.Subst.updateAll'_cons, Runtime.Subst.updateAll'_nil_left,
-                  Runtime.Subst.update']
-      iexact Hwp
-    · iexists v
-      isplitr
-      · ipure_intro; rfl
-      · iexact Hv
+    iapply (wp.fix (Φ := fun _ => emp) (vs := [v]))
+    simp only [Runtime.Subst.update', Runtime.Subst.updateAll'_cons,
+               Runtime.Subst.updateAll'_nil_left]
+    iexact Hv
   · iexact Hbound
 
 /-- Applying a single-argument lambda `(fun b -> body)` to a value reduces to substituting. -/
@@ -187,14 +180,7 @@ theorem wp.app_lambda_single {b : Runtime.Binder} {body : Runtime.Expr} {v : Run
   simp only [wps_cons, wps_nil]
   iapply wp.val
   iapply wp.func
-  iapply (@wp.fix .none [b] body Φ
-    (fun vs => ∃ v', ⌜vs = [v']⌝ ∗ wp (body.subst (Runtime.Subst.id.update' b v')) Φ))
-  · iintro _IH %vs ⟨%v', %Heq, Hwp'⟩
-    subst Heq
-    simp only [Runtime.Subst.updateAll'_cons, Runtime.Subst.updateAll'_nil_left,
-               Runtime.Subst.update']
-    iexact Hwp'
-  · iexists v
-    isplitr
-    · ipure_intro; rfl
-    · iexact Hwp
+  iapply (wp.fix (Φ := fun _ => emp) (vs := [v]))
+  simp only [Runtime.Subst.update', Runtime.Subst.updateAll'_cons,
+             Runtime.Subst.updateAll'_nil_left]
+  iexact Hwp
